trying to debug a proof

lib/steel/pulse/Pulse.Checker.Bind.fst
@@ -15,16 +15,16 @@ module LN = Pulse.Typing.LN
 module Metatheory = Pulse.Typing.Metatheory
 
 #push-options "--query_stats --ifuel 2 --z3rlimit_factor 4"
-let  mk_bind' (g:env)
+assume val  mk_bind' (g:env)
                 (pre:term)
                 (e1:st_term)
                 (e2:st_term)
                 (c1:comp_st)
                 (c2:comp_st)
                 (px:nvar { ~ (Set.mem (snd px) (dom g)) })
-                (d_e1:st_typing g e1 c1)
-                (d_c1res:tot_typing g (comp_res c1) (tm_type (comp_u c1)))
-                (d_e2:st_typing (push_binding g (snd px) (fst px) (comp_res c1)) (open_st_term_nv e2 px) c2)
+                ($d_e1:st_typing g e1 c1)
+                ($d_c1res:tot_typing g (comp_res c1) (tm_type (comp_u c1)))
+                ($d_e2:st_typing (push_binding g (snd px) (fst px) (comp_res c1)) (open_st_term_nv e2 px) c2)
                 (post_hint:post_hint_opt g { comp_post_matches_hint c2 post_hint })
                 (_:squash (
                     let _, x = px in
@@ -33,15 +33,15 @@ let  mk_bind' (g:env)
                     (~(x `Set.mem` freevars_st e2)) /\
                     open_term (comp_post c1) x == comp_pre c2))
   : T.Tac (checker_result_t g pre post_hint)
-   =  let _,x  = px in
-      let s2 = st_comp_of_comp c2 in
-      if x `Set.mem` freevars s2.post
-      then fail g None (Printf.sprintf "Bound variable %d escapes scope in postcondition %s" x (P.term_to_string s2.post))
-      else ( 
-        let res_typing, post_typing = bind_res_and_post_typing g s2 x post_hint  in
-        let (| t, c, d |) = mk_bind g pre e1 e2 c1 c2 px d_e1 d_c1res d_e2 res_typing post_typing in
-        (| t, c, d |)
-      )
+  //  =  let _,x  = px in
+  //     let s2 = st_comp_of_comp c2 in
+  //     if x `Set.mem` freevars s2.post
+  //     then fail g None (Printf.sprintf "Bound variable %d escapes scope in postcondition %s" x (P.term_to_string s2.post))
+  //     else ( 
+  //       let res_typing, post_typing = bind_res_and_post_typing g s2 x post_hint  in
+  //       let (| t, c, d |) = mk_bind g pre e1 e2 c1 c2 px d_e1 d_c1res d_e2 res_typing post_typing in
+  //       (| t, c, d |)
+  //     )
 
 #push-options "--z3rlimit_factor 8 --fuel 2 --ifuel 2 --query_stats"
 let check_bind
@@ -121,9 +121,10 @@ let check_tot_bind g t pre pre_typing post_hint check =
        c,
        T_TotBind _ _ e2_closed _ _ x (E e1_typing) e2_typing |)
 
+irreducible
 let coerce_eq (#a #b:Type) (x:a) (_:squash (a == b)) : y:b{y == x} = x
 
-let check_stapp_no_ctxt (g:env) (t:st_term { Tm_STApp? t.term })
+let check_stapp_no_ctxt (g:env) (t:st_term)
   : T.Tac (uvs : env { disjoint uvs g } &
            t:st_term &
            c:comp_st &
@@ -132,7 +133,7 @@ let check_stapp_no_ctxt (g:env) (t:st_term { Tm_STApp? t.term })
 module PS = Pulse.Prover.Substs
 open Pulse.Prover.Common
 open Pulse.Prover
-#push-options "--z3rlimit_factor 8 --fuel 1 --ifuel 1"
+#push-options "--z3rlimit_factor 8 --fuel 1 --ifuel 1 --admit_smt_queries true" // --admit_smt_queries true --debug Pulse.Checker.Bind --debug_level NormTop --ugly"
 let check_bindv2
   (g:env)
   (t:st_term {Tm_Bind? t.term})
@@ -144,8 +145,6 @@ let check_bindv2
 
   let Tm_Bind { binder=b; head=e1; body=e2 } = t.term in
 
-  match e1.term with
-  | Tm_STApp _ ->
     let (| uvs, e1, c1, d1 |) = check_stapp_no_ctxt g e1 in
     let c10 = c1 in
     // magic is comp_pre c1 typing, get from inversion of d1 
@@ -156,40 +155,60 @@ let check_bindv2
     // TODO: if the binder is annotated, check subtyping
     let g2 = push_binding g1 x b.binder_ppname (PS.nt_subst_term (comp_res c1) ss1) in
     let pre_e2 = open_term_nv (PS.nt_subst_term (comp_post c1) ss1) px * remaining_pre in
-    assert (g2 `env_extends` g1);
-    assert (g2 `env_extends` g);
+    // assert (g2 `env_extends` g1);
+    // assert (g2 `env_extends` g);
     // magic is the typing of pre_e2 in g2
     // remaining_pre is well-typed, may be prove function can return it?
     // well-typedness of open_term?
+    let post_hint2 : post_hint_opt g2 = extend_post_hint_opt_g g post_hint g2 in
     let (| e2, c2, d2 |) =
-      check g2 (open_st_term_nv e2 px) pre_e2 (magic ()) (extend_post_hint_opt_g g post_hint g2) in
+      check g2 (open_st_term_nv e2 px) pre_e2 (magic ()) post_hint2 in
     
-    if not (stateful_comp c2)
-    then fail g None "Bind: c2 is not st"
-    else
-      let d1 = st_typing_weakening g uvs e1 c1 d1 g1 in
-      let d1 = st_typing_weakening_end g1 uvs e1 c1 d1 uvs1 in
-      let d1 = PS.st_typing_nt_substs_derived g1 uvs1 #e1 #c1 d1 ss1 in
-      // if None? d1opt then fail g None "Bind: could not find a well-typed substitution"
-      // else
-        // g1 |- ss1 e1 : ss1 c1
-      let (| e1, c1, d1 |) = add_frame d1 #remaining_pre (magic ()) in
-      assert (comp_pre c1 == PS.nt_subst_term (comp_pre c10) ss1 * remaining_pre);
-      assert (comp_res c1 == PS.nt_subst_term (comp_res c10) ss1);
-      assert (None? (lookup g1 x));
-      assert (comp_post c1 == PS.nt_subst_term (comp_post c10) ss1 * remaining_pre);
-      assume (open_term remaining_pre x == remaining_pre);
-      assert (open_term (comp_post c1) x == comp_pre c2);
-   
-      let e2_closed = close_st_term e2 x in
-      assume (open_st_term e2_closed x == e2);
-      let d1 : st_typing g1 e1 c1 = coerce_eq d1 () in
-      let d2
-        : st_typing (push_binding g1 (snd px) (fst px) (comp_res c1)) (open_st_term_nv e2_closed px) c2
-        = coerce_eq d2 () in
-      // let r = mk_bind' g1 (comp_pre c1) e1 e2_closed c1 c2 px d1 (magic ()) d2 post_hint () in
+    // if not (stateful_comp c2) then fail g None "Bind: c2 is not st";
+    // let d1 = st_typing_weakening g uvs e1 c1 d1 g1 in
+    // let d1 = st_typing_weakening_end g1 uvs e1 c1 d1 uvs1 in
+    // let d1
+    //   : st_typing g1 (PS.nt_subst_st_term e1 ss1)
+    //                  (PS.nt_subst_comp c1 ss1) = PS.st_typing_nt_substs_derived g1 uvs1 #e1 #c1 d1 ss1 in
+    let d1
+      : st_typing g1 (PS.nt_subst_st_term e1 ss1)
+                     (PS.nt_subst_comp c1 ss1) = magic () in
 
+        // g1 |- ss1 e1 : ss1 c1
+    let (| e1, c1, d1 |) = add_frame d1 #remaining_pre (magic ()) in
+    // assert (comp_pre c1 == PS.nt_subst_term (comp_pre c10) ss1 * remaining_pre);
+    // assert (comp_res c1 == PS.nt_subst_term (comp_res c10) ss1);
+    // assert (None? (lookup g1 x));
+    // assert (comp_post c1 == PS.nt_subst_term (comp_post c10) ss1 * remaining_pre);
+    // assume (open_term remaining_pre x == remaining_pre);
+    // assert (open_term (comp_post c1) x == comp_pre c2);
+   
+    let e2_closed = close_st_term e2 x in
+    // assume (open_st_term e2_closed x == e2);
+    // let d1 : st_typing g1 e1 c1 = coerce_eq d1 () in
+    // let d2
+    //   : st_typing (push_binding g1 (snd px) (fst px) (comp_res c1)) (open_st_term_nv e2_closed px) c2
+    //   = coerce_eq d2 () in
+    // let post_hint1 : post_hint_opt g1 = extend_post_hint_opt_g g post_hint g1 in
+    // assume (comp_post_matches_hint c2 post_hint1);
+    // assume (stateful_comp c1);
+    // assume (~ (x `Set.mem` freevars_st e2_closed));
+    // let g : env = g1 in
+    // let pre : term = comp_pre c1 in
+    // let e1 : st_term = e1 in
+    // let e2 : st_term = e2_closed in
+    // let c1 : comp_st = c1 in
+    // let c2 : comp_st = c2 in
+    // let px : px:nvar { ~ (Set.mem (snd px) (dom g)) } = px in
+    // let d_e1 : st_typing g e1 c1 = coerce_eq d1 () in
+    // let d_c1res : tot_typing g (comp_res c1) (tm_type (comp_u c1)) = magic () in
+    // let d_e2 : st_typing (push_binding g (snd px) (fst px) (comp_res c1)) (open_st_term_nv e2 px) c2 =
+    //   coerce_eq d2 () in
+    // let post_hint : post_hint:post_hint_opt g { comp_post_matches_hint c2 post_hint } = magic () in
+
+    // let r = mk_bind' g pre e1 e2 c1 c2 px d_e1 d_c1res d_e2 post_hint () in
+    let r =
+      mk_bind' g1 (magic ()) e1 e2_closed c1 c2 px (magic ()) (magic ()) (magic ()) (magic ()) () in
       // k post_hint r
-      admit ()
-  | _ -> fail g None "Bind: e1 is not an stapp"
+    admit ()
 #pop-options
